Numbers/Notation.lean
@@ -13,13 +13,13 @@ scoped syntax "s32%" num : term
 scoped syntax "s64%" num : term
 
 macro_rules
-| `(u8% $n:num)  => `(Unsigned.ofNat (n := ⟨8, by decide⟩)  $n)
-| `(u16% $n:num) => `(Unsigned.ofNat (n := ⟨16, by decide⟩) $n)
-| `(u32% $n:num) => `(Unsigned.ofNat (n := ⟨32, by decide⟩) $n)
-| `(u64% $n:num) => `(Unsigned.ofNat (n := ⟨64, by decide⟩) $n)
+| `(u8% $n:num)  => `(Unsigned.ofNat (n := 8)  $n)
+| `(u16% $n:num) => `(Unsigned.ofNat (n := 16) $n)
+| `(u32% $n:num) => `(Unsigned.ofNat (n := 32) $n)
+| `(u64% $n:num) => `(Unsigned.ofNat (n := 64) $n)
 
 macro_rules
-| `(s8% $n:num)  => `(Signed.ofNat (n := ⟨8, by decide⟩)  $n)
-| `(s16% $n:num) => `(Signed.ofNat (n := ⟨16, by decide⟩) $n)
-| `(s32% $n:num) => `(Signed.ofNat (n := ⟨32, by decide⟩) $n)
-| `(s64% $n:num) => `(Signed.ofNat (n := ⟨64, by decide⟩) $n)
+| `(s8% $n:num)  => `(Signed.ofNat (n := 8)  $n)
+| `(s16% $n:num) => `(Signed.ofNat (n := 16) $n)
+| `(s32% $n:num) => `(Signed.ofNat (n := 32) $n)
+| `(s64% $n:num) => `(Signed.ofNat (n := 64) $n)
